theories/DiophantineConstraints/Reductions/FRACTRAN_to_H10C_SAT.v
@@ -7,9 +7,9 @@
 (*         CeCILL v2 FREE SOFTWARE LICENSE AGREEMENT          *)
 (**************************************************************)
 
-Require Import Arith Omega Max.
-Require Import Undecidability.Shared.Prelim.
-From Undecidability Require Import ILL.Definitions.
+Require Import List Arith Omega Max.
+
+Require Import Undecidability.Synthetic.Undecidability.
 
 From Undecidability Require Import Shared.Libs.DLW.Utils.utils H10.Dio.dio_logic H10.Dio.dio_elem.
 From Undecidability Require Import H10.FRACTRAN_DIO Problems.FRACTRAN.
