theories/FRACTRAN/FRACTRAN_undec.v
@@ -9,27 +9,24 @@
 (*         CeCILL v2 FREE SOFTWARE LICENSE AGREEMENT          *)
 (**************************************************************)
 
-(* From Undecidability Require Import ILL.Definitions. *)
-From Undecidability.BinaryStackMachines  Require Import BSM BSM_undec.
-From Undecidability.MinskyMachines       Require Import MM BSM_MM.
-From Undecidability.ILL.Ll               Require Import eill ill.
-
-From Undecidability.ILL Require Import MM_EILL EILL_ILL.
-
 Require Import Undecidability.Synthetic.Undecidability.
 
-Check BSM_MM_HALTS_ON_ZERO.
-Check BSM_MM_HALTING.
+From Undecidability.MinskyMachines
+  Require Import MM MM_undec.
 
-Theorem EILL_undec : undecidable EILL_PROVABILITY.
+From Undecidability.FRACTRAN
+  Require Import FRACTRAN Reductions.MM_FRACTRAN.
+
+Theorem FRACTRAN_REG_undec : undecidable FRACTRAN_REG_HALTING.
 Proof.
-  apply (undecidability_from_reducibility BSM_undec).
-  eapply reduces_transitive. exact BSM_MM_HALTS_ON_ZERO.
-  exact MM_HALTS_ON_ZERO_EILL_PROVABILITY.
+  apply (undecidability_from_reducibility MM_HALTING_undec).
+  apply MM_FRACTRAN_REG_HALTING.
 Qed.
 
-Theorem ILL_undec : undecidable ILL_PROVABILITY.
+Check FRACTRAN_REG_undec.
+
+Theorem FRACTRAN_undec : undecidable FRACTRAN_HALTING.
 Proof.
-  apply (undecidability_from_reducibility EILL_undec).
-  exact EILL_ILL_PROVABILITY.
+  apply (undecidability_from_reducibility FRACTRAN_REG_undec).
+  apply FRACTRAN_REG_FRACTRAN_HALTING.
 Qed.
