theories/MinskyMachines/MM/mm_no_self.v
@@ -16,7 +16,7 @@ From Undecidability.Shared.Libs.DLW
   Require Import Utils.utils Vec.pos Vec.vec
                  Code.subcode Code.sss.
 
-From Undecidability.MinskyMachines
+From Undecidability.MinskyMachines.MM
   Require Import mm_defs.
 
 Set Implicit Arguments.
