theories/MinskyMachines/MMA2_undec.v
@@ -1,0 +1,21 @@
+(**************************************************************)
+(*   Copyright Dominique Larchey-Wendling [*]                 *)
+(*                                                            *)
+(*                             [*] Affiliation LORIA -- CNRS  *)
+(**************************************************************)
+(*      This file is distributed under the terms of the       *)
+(*         CeCILL v2 FREE SOFTWARE LICENSE AGREEMENT          *)
+(**************************************************************)
+
+Require Import Undecidability.Synthetic.Undecidability.
+
+From Undecidability.FRACTRAN Require Import FRACTRAN FRACTRAN_undec.
+From Undecidability.MinskyMachines Require Import MM FRACTRAN_to_MMA2.
+
+Lemma MMA2_HALTING_undec : undecidable MMA2_HALTING.
+Proof.
+  apply (undecidability_from_reducibility FRACTRAN_REG_undec).
+  apply FRACTRAN_REG_MMA2_HALTING.
+Qed.
+
+Check MMA2_HALTING_undec.
