theories/MinskyMachines/Reductions/MUREC_MM.v
@@ -1,0 +1,47 @@
+(**************************************************************)
+(*   Copyright Dominique Larchey-Wendling [*]                 *)
+(*                                                            *)
+(*                             [*] Affiliation LORIA -- CNRS  *)
+(**************************************************************)
+(*      This file is distributed under the terms of the       *)
+(*         CeCILL v2 FREE SOFTWARE LICENSE AGREEMENT          *)
+(**************************************************************)
+
+Require Import List Arith Omega.
+
+Require Import Undecidability.Synthetic.Undecidability.
+
+From Undecidability.Shared.Libs.DLW 
+  Require Import pos vec sss.
+
+From Undecidability.MinskyMachines
+  Require Import MM.
+
+From Undecidability.MuRec 
+  Require Import recalg ra_simul.
+
+Local Notation "'⟦' f '⟧'"  := (@ra_rel _ f) (at level 0).
+Local Notation "P /MM/ s ↓" := (sss_terminates (@mm_sss _) P s) (at level 70, no associativity).
+
+Section MUREC_MM_HALTING.
+
+ Let f : MUREC_PROBLEM -> MM_PROBLEM.
+  Proof.
+    intros g.
+    destruct (ra_mm_simulator g) as (m & P & _).
+    exists (S m), P; apply vec_zero.
+  Defined.
+
+  Theorem MUREC_MM_HALTING : MUREC_HALTING ⪯ MM_HALTING.
+  Proof.
+    exists f; unfold f.
+    intros g; simpl; unfold MUREC_HALTING, MM_HALTING.
+    destruct (ra_mm_simulator g) as (m & P & H); simpl.
+    rewrite H, vec_app_nil; tauto.
+  Qed.
+
+End MUREC_MM_HALTING.
+
+(* Check MUREC_MM_HALTING. *)
+(* Print Assumptions MUREC_MM_HALTING. *)
+
