theories/MinskyMachines/Reductions/PCPb_to_MM.v
@@ -1,0 +1,28 @@
+(**************************************************************)
+(*   Copyright Dominique Larchey-Wendling [*]                 *)
+(*                                                            *)
+(*                             [*] Affiliation LORIA -- CNRS  *)
+(**************************************************************)
+(*      This file is distributed under the terms of the       *)
+(*         CeCILL v2 FREE SOFTWARE LICENSE AGREEMENT          *)
+(**************************************************************)
+
+Require Import Undecidability.Synthetic.Undecidability.
+
+From Undecidability.PCP                  Require Import PCP PCPb_iff_iPCPb.
+From Undecidability.BinaryStackMachines  Require Import BSM iBPCP_BSM.
+From Undecidability.MinskyMachines       Require Import MM BSM_MM.
+ 
+Theorem PCPb_MM_HALTS_ON_ZERO : PCPb ⪯ MM_HALTS_ON_ZERO.
+Proof.
+  eapply reduces_transitive. exact PCPb_iff_iPCPb.reductionLR.
+  eapply reduces_transitive. exact iBPCP_BSM_HALTING.
+  apply BSM_MM_HALTS_ON_ZERO.
+Qed.
+
+Theorem PCPb_MM_HALTING : PCPb ⪯ MM_HALTING.
+Proof.
+  eapply reduces_transitive. exact PCPb_iff_iPCPb.reductionLR.
+  eapply reduces_transitive. exact iBPCP_BSM_HALTING.
+  apply BSM_MM_HALTING.
+Qed.
