theories/PCP/Reductions/HALT_TM1_to_PCPb.v
@@ -9,6 +9,10 @@
 
 (* Direct reductions from Halting of 1-TM to binary PCP *)
 
+Require Import List.
+
+Import ListNotations.
+
 Require Import Undecidability.Synthetic.Undecidability.
 
 Require Import Undecidability.TM.Halting.
@@ -20,7 +24,24 @@ From Undecidability.PCP
   Require Import PCP.
 
 From Undecidability.PCP.Reductions
-  Require Import SR_to_MPCP MPCP_to_PCP PCP_to_PCPb.
+  Require Import SR_to_MPCP MPCP_to_PCP PCP_to_PCPb PCPb_iff_iPCPb.
+
+Notation "p '⪯c' q 'by' l" := (@reduction_chain _ _ p q l) (at level 70).
+
+(*
+Check singleTM.TM_conv.
+Check Halt_SRH.
+Check SRH_to_SR.reduction.
+Check SR_to_MPCP.reduction.
+
+Check SR.SRH.
+
+Lemma HALT_TM1_chain_PCP : HaltTM 1 ⪯c PCP by [⎩singleTM.Halt⎭;
+                                              ⎩SR.SRH⎭;
+                                              ⎩SR.SR⎭;
+                                              ⎩MPCP⎭;
+                                              ⎩PCP⎭].
+*)
 
 Lemma HALT_TM1_to_PCP : HaltTM 1 ⪯ PCP.
 Proof.
@@ -35,4 +56,10 @@ Lemma HALT_TM1_to_PCPb : HaltTM 1 ⪯ PCPb.
 Proof.
   eapply reduces_transitive. exact HALT_TM1_to_PCP.
   exact PCP_to_PCPb.reduction.
+Qed.
+
+Lemma HALT_TM1_to_iPCPb : HaltTM 1 ⪯ iPCPb.
+Proof.
+  eapply reduces_transitive. exact HALT_TM1_to_PCPb.
+  exact PCPb_iff_iPCPb.reductionLR.
 Qed.
