theories/Problems/BSM.v
@@ -1,8 +1,8 @@
-From Undecidability.BinaryStackMachines Require Export bsm_defs bsm_utils.
+From Undecidability.BinaryStackMachines Require Export BSM.
 
 (* The halting problem for binary stack machines *)
 
 (* Certified Undecidability of Intuitionistic Linear Logic via Binary Stack Machines and Minsky Machines. Yannick Forster and Dominique Larchey-Wendling. CPP '19. http://uds-psl.github.io/ill-undecidability/ *)
 
-About BSM_HALTING. (* Halting problem for Minsky machines *)
+About BSM_HALTING. (* Halting problem for Binary Stack machines machines *)
 
