theories/Reductions/PCPb_to_MM.v
@@ -1,0 +1,1 @@
+From Undecidability.MinskyMachines Require Export PCPb_to_MM.
